\documentclass{article}
\usepackage{amsmath}
\begin{document}

To solve the quadratic equation:
\[
3x^2 - 7x + 2 = 0
\]

We use the quadratic formula:
\[
x = \frac{-b \pm \sqrt{b^2 - 4ac}}{2a}
\]

Given: \(a = 3\), \(b = -7\), \(c = 2\)

\[
x = \frac{-(-7) \pm \sqrt{(-7)^2 + 4 \cdot 3 \cdot 2}}{2 \cdot 3}
\]

\[
x = \frac{7 \pm \sqrt{49 + 24}}{6}
\]

\[
x = \frac{7 \pm \sqrt{73}}{6}
\]

So the solutions are:
\[
x_1 = \frac{7 + \sqrt{73}}{6}, \quad x_2 = \frac{7 - \sqrt{73}}{6}
\]

\end{document}
